test/test_add_context.v
@@ -1,12 +1,14 @@
+From stdpp Require Import bitvector.definitions.
 From Stdlib Require Import BinInt Bits.
 Require Import quartz.lang.Syntax. Import type.
 Import (notations) type expr eexpr.
 
-Definition test_add_context_inner {var} := @fn.Fn var type.Unit (Bits 16%Z) (fun _ =>
+Definition test_add_context_inner {var} := @fn.Fn var type.Unit (Bits 16%N) (fun _ =>
     quartz_eexpr:(
-      let a := $(expr.Const (t:=Bits 8%Z) (bits.of_Z _ 255)) in
-      let b := $(expr.Const (t:=Bits 8%Z) (bits.of_Z _ 1)) in
-      return $(expr.Unop (t1:=Bits _%Z) (@unop.Resize false _ 16%Z) quartz_expr:(#a + #b))
+      let a := $(expr.Const (t:=Bits 8) (Z_to_bv _ 255)) in
+      let b := $(expr.Const (t:=Bits 8) (Z_to_bv _ 1)) in
+      return $(expr.Unop (t1:=Bits _) (@unop.Resize false _ 16) quartz_expr:(#a + #b))
     )).
 
 Definition test_add_context {var fn} := fns.package_global_fns'' var fn (@test_add_context_inner).
+
