test/test_array_of_arrays.v
@@ -1,14 +1,14 @@
-From Stdlib Require Import BinInt Bits.
+From stdpp Require Import bitvector.definitions.
+From Stdlib Require Import BinInt.
 Require Import quartz.lang.Syntax. Import type.
 Import (notations) type expr eexpr.
-
-Definition test_array_of_arrays_inner {var} := @fn.Fn var type.Unit (Array (Array (Bits 32%Z) 3%nat) 2%nat) (fun _ => quartz_eexpr:(
-  let arr := $(expr.Const (t:=Array (Array (Bits 32%Z) 3%nat) 2%nat) (Vector.const (Vector.const (bits.of_Z _ 42%Z) 3%nat) 2%nat)) in
-  let i := $(expr.Const (t:=Bits 1%Z) (bits.of_Z _ 1%Z)) in
-  let j := $(expr.Const (t:=Bits 2%Z) (bits.of_Z _ 2%Z)) in
+Definition test_array_of_arrays_inner {var} := @fn.Fn var type.Unit (Array (Array (Bits 32) 3%nat) 2%nat) (fun _ => quartz_eexpr:(
+  let arr := $(expr.Const (t:=Array (Array (Bits 32%N) 3%nat) 2%nat) (Vector.const (Vector.const (Z_to_bv _ 42%Z) 3%nat) 2%nat)) in
+  let i := $(expr.Const (t:=Bits 1) (Z_to_bv _ 1%Z)) in
+  let j := $(expr.Const (t:=Bits 2) (Z_to_bv _ 2%Z)) in
   let inner_arr := #arr[#i] in
   let cur_val := #inner_arr[#j] in
-  let next_val := #cur_val + $(expr.Const (t:=Bits 32%Z) (bits.of_Z _ 1%Z)) in
+  let next_val := #cur_val + $(expr.Const (t:=Bits 32) (Z_to_bv _ 1%Z)) in
   let inner_arr_new <- #inner_arr[#j] = #next_val in
   let arr_new <- #arr[#i] = #inner_arr_new in
   return #arr_new)).
